To reduce the given equation to the form ( a \cdot t^2 + B \cdot t + c = 0 ), let's break it down step by step.

Original Equation
The equation is:

[ \left[ x_0 + \left( (X_e + t X_D - x_0) X_q + (Y_e + t Y_D - y_0) Y_q + (Z_e + t Z_D - z_0) Z_q \right) X_q - x \right]^2 + \left[ y_0 + \left( (X_e + t X_D - x_0) X_q + (Y_e + t Y_D - y_0) Y_q + (Z_e + t Z_D - z_0) Z_q \right) Y_q - y \right]^2 + \left[ z_0 + \left( (X_e + t X_D - x_0) X_q + (Y_e + t Y_D - y_0) Y_q + (Z_e + t Z_D - z_0) Z_q \right) Z_q - z \right]^2 - R^2 = 0 ]

Where:

( X_e, Y_e, Z_e ): Ray origin coordinates
( X_D, Y_D, Z_D ): Ray direction components
( x_0, y_0, z_0 ): Cylinder base coordinates
( X_q, Y_q, Z_q ): Cylinder axis direction components (normalized)
( R ): Cylinder radius
( t ): Parameter for the ray equation
Step 1: Substitute the ray equation
The ray equation is: [ P(t) = (X_e + t X_D, Y_e + t Y_D, Z_e + t Z_D) ]

Substitute ( P(t) ) into the cylinder equation: [ \left[ x_0 + \left( (X_e + t X_D - x_0) X_q + (Y_e + t Y_D - y_0) Y_q + (Z_e + t Z_D - z_0) Z_q \right) X_q - x \right]^2 + \left[ y_0 + \left( (X_e + t X_D - x_0) X_q + (Y_e + t Y_D - y_0) Y_q + (Z_e + t Z_D - z_0) Z_q \right) Y_q - y \right]^2 + \left[ z_0 + \left( (X_e + t X_D - x_0) X_q + (Y_e + t Y_D - y_0) Y_q + (Z_e + t Z_D - z_0) Z_q \right) Z_q - z \right]^2 - R^2 = 0 ]

Step 2: Simplify the projection onto the cylinder axis
Let: [ L = (X_e - x_0, Y_e - y_0, Z_e - z_0) ]

The projection of ( P(t) ) onto the cylinder axis is: [ P_{\text{proj}} = (L + t D) \cdot Q ]

Where:

( D = (X_D, Y_D, Z_D) ): Ray direction
( Q = (X_q, Y_q, Z_q) ): Cylinder axis direction
Thus: [ P_{\text{proj}} = (L \cdot Q) + t (D \cdot Q) ]

Step 3: Decompose the equation
The distance from the ray to the cylinder axis is: [ \text{Distance}^2 = | (L + t D) - P_{\text{proj}} Q |^2 ]

Substitute ( P_{\text{proj}} ): [ \text{Distance}^2 = | (L + t D) - \left[ (L \cdot Q) + t (D \cdot Q) \right] Q |^2 ]

Expand: [ \text{Distance}^2 = | L + t D - (L \cdot Q) Q - t (D \cdot Q) Q |^2 ]

Group terms: [ \text{Distance}^2 = | (L - (L \cdot Q) Q) + t (D - (D \cdot Q) Q) |^2 ]

Let: [ L_{\perp} = L - (L \cdot Q) Q ] [ D_{\perp} = D - (D \cdot Q) Q ]

Thus: [ \text{Distance}^2 = | L_{\perp} + t D_{\perp} |^2 ]

Step 4: Expand the quadratic form
Expand the norm: [ \text{Distance}^2 = (L_{\perp} \cdot L_{\perp}) + 2t (L_{\perp} \cdot D_{\perp}) + t^2 (D_{\perp} \cdot D_{\perp}) ]

Subtract the cylinder radius squared: [ \text{Distance}^2 - R^2 = 0 ]

Step 5: Identify coefficients
Compare with ( a \cdot t^2 + B \cdot t + c = 0 ):

( a = D_{\perp} \cdot D_{\perp} )
( B = 2 (L_{\perp} \cdot D_{\perp}) )
( c = (L_{\perp} \cdot L_{\perp}) - R^2 )
Final Form
[ a = D_{\perp} \cdot D_{\perp} ] [ B = 2 (L_{\perp} \cdot D_{\perp}) ] [ c = (L_{\perp} \cdot L_{\perp}) - R^2 ]

Where:

( L_{\perp} = L - (L \cdot Q) Q )
( D_{\perp} = D - (D \cdot Q) Q )